Code/Prelude/Lexico.v
@@ -1,0 +1,82 @@
+Require Import Wellfounded.
+Require Import CompatibleRelation.
+
+Section Lexico.
+  Context (X : CompatRel)
+          {Y : Type}
+          `{isCompatRel X}
+          (RY : Y -> Y -> Prop).
+  
+  Definition lexico
+    : X * Y -> X * Y -> Prop
+    := fun x y => fst x > fst y
+                  \/
+                  fst x >= fst y /\ RY (snd x) (snd y).
+
+  Proposition lexico_trans
+              (RYtrans : forall (y1 y2 y3 : Y),
+                  RY y1 y2 -> RY y2 y3 -> RY y1 y3)
+              {x y z : X * Y}
+              (p : lexico x y)
+              (q : lexico y z)
+    : lexico x z.
+  Proof.
+    destruct p as [p | [p1 p2]], q as [q | [q1 q2]].
+    - left.
+      exact (gt_trans p q).
+    - left.
+      exact (gt_ge p q1).
+    - left.
+      exact (ge_gt p1 q).
+    - right.
+      split.
+      + exact (ge_trans p1 q1).
+      + exact (RYtrans _ _ _ p2 q2).
+  Qed.
+  
+  Proposition lexico_Wf_help
+              (x : X * Y)
+              (z1 : X)
+              (p : fst x >= z1)
+              (HX : isWf lexico x)
+    : isWf lexico (z1 , snd x).
+  Proof.
+    revert p.
+    revert z1.
+    induction HX as [[q1 q2] Hq IHq].
+    simpl in *.
+    intros z1 p.
+    apply acc.
+    intros [w1 w2] [H' | [H1 H2]] ; simpl in *.
+    - refine (IHq (w1 , w2) _ w1 _) ; simpl.
+      + left ; simpl.
+        exact (ge_gt p H').
+      + apply ge_refl.
+    - refine (IHq (q1 , w2) _ w1 _).
+      + right ; simpl.
+        split.
+        * apply ge_refl.
+        * exact H2.
+      + refine (ge_trans p H1).
+  Qed.
+
+  Proposition lexico_Wf
+              (HX : Wf (fun (x y : X) => x > y))
+              (HY : Wf RY)
+    : Wf lexico.
+  Proof.
+    intros [x y].
+    pose (HX x) as Hx.
+    revert y.
+    induction Hx as [x Hx IHx].
+    intros y.
+    pose (HY y) as Hy.
+    induction Hy as [y Hy IHy].
+    apply acc.
+    intros [z1 z2] [Hz | [Hz1 Hz2]] ; simpl in *.
+    - apply IHx.
+      exact Hz.
+    - refine (lexico_Wf_help (x , _) z1 Hz1 _).
+      exact (IHy z2 Hz2).
+  Qed.
+End Lexico.
